Worked through AdvanceFlits

model/noc2.dfy
@@ -1,4 +1,6 @@
 module NoC2 {
+  import Std.Collections.Seq
+
   datatype Channel =
     | Channel(buffer: seq<nat>, isEmpty: bool, isFull: bool)
     {
@@ -21,9 +23,39 @@ module NoC2 {
       {
         Channel(this.buffer, this.length() == 0, this.length() >= buffer_length)
       }
+
+      function dropFirst(): Channel
+        requires this.length() > 0
+      {
+        Channel(Seq.DropFirst(this.buffer), this.isEmpty, this.isFull)
+      }
+
+      function peekFirst(): nat
+        requires this.length() > 0
+      {
+        this.buffer[0]
+      }
     }
 
   type FixedSeq<T> = i: seq<T> | |i| == 5 witness *
+
+  datatype Direction =
+    | North
+    | East
+    | South
+    | West
+    | Local
+    {
+      function getDestinationDir(): Direction
+        requires !this.Local?
+      {
+        match this
+        case North => South
+        case South => North
+        case East => West
+        case West => East
+      }
+    }
 
   const N := 0
   const E := 1
@@ -31,88 +63,232 @@ module NoC2 {
   const W := 3
   const L := 4
 
+  class ChannelWrapper<T> {
+    var north: T
+    var east:  T
+    var south: T
+    var west:  T
+    var local: T
+
+    constructor(north: T, east: T, south: T, west: T, local: T)
+      ensures this.north == north
+      ensures this.east  == east
+      ensures this.south == south
+      ensures this.west  == west
+      ensures this.local == local
+    {
+      this.north := north;
+      this.east  := east;
+      this.south := south;
+      this.west  := west;
+      this.local := local;
+    }
+
+    function asSeq(): (s: seq<T>)
+      reads this
+      ensures |s| == 5
+    {
+      [this.north, this.east, this.south, this.west, this.local]
+    }
+
+    function fromDir(dir: Direction): T
+      reads this`north
+      reads this`east
+      reads this`south
+      reads this`west
+      reads this`local
+    {
+      match dir
+      case North => this.north
+      case East  => this.east
+      case South => this.south
+      case West  => this.west
+      case Local => this.local
+    }
+
+    method writeByDir(dir: Direction, data: T)
+      modifies this
+      ensures dir != North ==> old(this.north) == this.north
+      ensures dir != East  ==> old(this.east)  == this.east
+      ensures dir != South ==> old(this.south) == this.south
+      ensures dir != West  ==> old(this.west)  == this.west
+      ensures dir != Local ==> old(this.local) == this.local
+    {
+      match dir
+      case North => { this.north := data; }
+      case East  => { this.east  := data; }
+      case South => { this.south := data; }
+      case West  => { this.west  := data; }
+      case Local => { this.local := data; }
+    }
+  }
+
   class Router {
     const id: nat
     const dim: nat
     const buffer_length: nat
-    // var channels: FixedSeq<Channel>
-    var north: Channel
-    var east:  Channel
-    var south: Channel
-    var west:  Channel
-    var local: Channel
-    var serviced: FixedSeq<bool>
+    var channels: ChannelWrapper<Channel>
+    var serviced: ChannelWrapper<bool>
+    var used: ChannelWrapper<bool>
     var totalUnserviced: nat
 
+    predicate valid() {
+      && this.dim >= 2
+      && 0 <= this.id < this.dim*this.dim
+      && buffer_length > 0
+    }
 
     constructor(buffer_length: nat, id: nat, dim: nat)
+      requires buffer_length > 0
+      requires dim >= 2
+      requires 0 <= id < dim*dim
       ensures this.id == id
       ensures this.dim == dim
       ensures this.buffer_length == buffer_length
-      ensures this.north.length() == 0
-      ensures this.east.length()  == 0
-      ensures this.south.length() == 0
-      ensures this.west.length()  == 0
-      ensures this.local.length() == 0
-      ensures this.serviced == [false, false, false, false, false]
+      ensures this.channels.north.length() == 0
+      ensures this.channels.east.length()  == 0
+      ensures this.channels.south.length() == 0
+      ensures this.channels.west.length()  == 0
+      ensures this.channels.local.length() == 0
+      ensures this.serviced.asSeq() == [false, false, false, false, false]
       ensures this.totalUnserviced == 0
+      ensures this.used.asSeq() == [false, false, false, false, false]
+      ensures valid()
     {
       this.id := id;
       this.dim := dim;
       this.buffer_length := buffer_length;
-      this.north := Channel.init();
-      this.east  := Channel.init();
-      this.south := Channel.init();
-      this.west  := Channel.init();
-      this.local := Channel.init();
-      this.serviced := [false, false, false, false, false];
+      this.channels := new ChannelWrapper(Channel.init(), Channel.init(), Channel.init(), Channel.init(), Channel.init());
+      this.serviced := new ChannelWrapper(false, false, false, false, false);
+      this.used := new ChannelWrapper(false, false, false, false, false);
       this.totalUnserviced := 0;
     }
 
     static method getDestination(id: nat, dim: nat) returns (dest: nat)
       ensures {:axiom} 0 <= id < dim*dim && dest != id
 
-    method generateFlits(cycle: nat)
-      requires this.local.length() <= this.buffer_length
-      modifies this`local
-      ensures old(this.local.buffer) <= this.local.buffer
-      ensures this.local.length() <= this.buffer_length 
+    function column(): nat
+      requires valid()
     {
-      if cycle % 3 < 3 && |this.local.buffer| < this.buffer_length {
+      Router.column_s(this.id, this.dim)
+    }
+
+    static function column_s(id: nat, dim: nat): nat
+      requires dim != 0
+    {
+      id % dim
+    }
+
+    function row(): nat
+      requires valid()
+    {
+      Router.row_s(id, dim)
+    }
+
+    static function row_s(id: nat, dim: nat): nat
+      requires dim != 0
+    {
+      id / dim
+    }
+
+    method generateFlits(cycle: nat)
+      requires valid()
+      requires this.channels.local.length() <= this.buffer_length
+      modifies this.channels`local
+      ensures old(this.channels.local.buffer) <= this.channels.local.buffer
+      ensures this.channels.local.length() <= this.buffer_length
+      ensures valid()
+    {
+      if cycle % 3 < 3 && |this.channels.local.buffer| < this.buffer_length {
         var dest := Router.getDestination(this.id, this.dim);
-        this.local := this.local.insert(dest);
+        this.channels.local := this.channels.local.insert(dest);
       }
     }
 
     method prepRouter(cycle: nat)
-      modifies this`north
-      modifies this`east
-      modifies this`south
-      modifies this`west
-      modifies this`local
-      ensures old(this.north.buffer) == this.north.buffer
-      ensures old(this.east.buffer)  == this.east.buffer
-      ensures old(this.south.buffer) == this.south.buffer
-      ensures old(this.west.buffer)  == this.west.buffer
-      ensures old(this.local.buffer) == this.local.buffer
-      ensures (this.north.length() == 0 <==> this.north.isEmpty) && (this.north.length() >= this.buffer_length <==> this.north.isFull)
-      ensures (this.east.length()  == 0 <==> this.east.isEmpty)  && (this.east.length()  >= this.buffer_length <==> this.east.isFull)
-      ensures (this.south.length() == 0 <==> this.south.isEmpty) && (this.south.length() >= this.buffer_length <==> this.south.isFull)
-      ensures (this.west.length()  == 0 <==> this.west.isEmpty)  && (this.west.length()  >= this.buffer_length <==> this.west.isFull)
-      ensures (this.local.length() == 0 <==> this.local.isEmpty) && (this.local.length() >= this.buffer_length <==> this.local.isFull)
+      requires valid()
+      modifies this.channels`north
+      modifies this.channels`east
+      modifies this.channels`south
+      modifies this.channels`west
+      modifies this.channels`local
+      ensures old(this.channels.north.buffer) == this.channels.north.buffer
+      ensures old(this.channels.east.buffer)  == this.channels.east.buffer
+      ensures old(this.channels.south.buffer) == this.channels.south.buffer
+      ensures old(this.channels.west.buffer)  == this.channels.west.buffer
+      ensures old(this.channels.local.buffer) == this.channels.local.buffer
+      ensures (this.channels.north.length() == 0 <==> this.channels.north.isEmpty) && (this.channels.north.length() >= this.buffer_length <==> this.channels.north.isFull)
+      ensures (this.channels.east.length()  == 0 <==> this.channels.east.isEmpty)  && (this.channels.east.length()  >= this.buffer_length <==> this.channels.east.isFull)
+      ensures (this.channels.south.length() == 0 <==> this.channels.south.isEmpty) && (this.channels.south.length() >= this.buffer_length <==> this.channels.south.isFull)
+      ensures (this.channels.west.length()  == 0 <==> this.channels.west.isEmpty)  && (this.channels.west.length()  >= this.buffer_length <==> this.channels.west.isFull)
+      ensures (this.channels.local.length() == 0 <==> this.channels.local.isEmpty) && (this.channels.local.length() >= this.buffer_length <==> this.channels.local.isFull)
+      ensures valid()
     {
-      this.north := this.north.setFlags(this.buffer_length);
-      this.east  := this.east.setFlags(this.buffer_length);
-      this.south := this.south.setFlags(this.buffer_length);
-      this.west  := this.west.setFlags(this.buffer_length);
-      this.local := this.local.setFlags(this.buffer_length);
+      this.channels.north := this.channels.north.setFlags(this.buffer_length);
+      this.channels.east  := this.channels.east.setFlags(this.buffer_length);
+      this.channels.south := this.channels.south.setFlags(this.buffer_length);
+      this.channels.west  := this.channels.west.setFlags(this.buffer_length);
+      this.channels.local := this.channels.local.setFlags(this.buffer_length);
     }
 
-    method send()
-      modifies this`serviced
-
+    method send(other: Router, from: Direction, dir: Direction)
+      requires valid()
+      requires this.dim == other.dim
+      requires this.id != other.dim
+      requires dir != Local
+      requires this.channels.fromDir(from).length() > 0
+      modifies this.serviced
+      modifies this.used
+      modifies this.channels
+      modifies this`totalUnserviced
+      modifies other.channels
+      ensures valid()
     {
+      var dest_dir := dir.getDestinationDir();
 
+      if !other.channels.fromDir(dest_dir).isFull && !this.used.fromDir(dir) {
+        // Send packet from source
+        var from_channel := this.channels.fromDir(from);
+        var packet := from_channel.peekFirst();
+        this.channels.writeByDir(from, from_channel.dropFirst());
+
+        // recieve packet at destination
+        other.channels.writeByDir(dest_dir, other.channels.fromDir(dest_dir).insert(packet));
+
+        // mark used
+        this.used.writeByDir(dir, true);
+        this.serviced.writeByDir(from, true);
+      } else {
+        this.totalUnserviced := this.totalUnserviced + 1;
+      }
+    }
+
+    method advanceFlits(other: Router, from: Direction)
+      requires valid()
+      requires this.dim == other.dim
+      requires this.id != other.dim
+      requires this.channels.fromDir(from).length() > 0
+      modifies this.serviced
+      modifies this.used
+      modifies this.channels
+      modifies this`totalUnserviced
+      modifies other.channels
+      ensures valid()
+    {
+      var dest_id := this.channels.fromDir(from).peekFirst();
+      var column_shift := Router.column_s(dest_id, this.dim) - this.column();
+
+      if column_shift == 0 {
+        if dest_id < this.id {
+          this.send(other, from, North);
+        } else {
+          this.send(other, from, South);
+        }
+      } else if column_shift < 0 {
+        this.send(other, from, West);
+      } else {
+        this.send(other, from, East);
+      }
     }
   }
 }
